cpSTLC/cpSTLCa_Props.v
@@ -30,8 +30,6 @@ Require Import ConceptParams.BasicPLDefs.Utils.
 Require Import ConceptParams.AuxTactics.LibTactics.
 Require Import ConceptParams.AuxTactics.BasicTactics.
 
-Require Import ConceptParams.ListAsAVL.ListAsSet.
-
 Require Import ConceptParams.cpSTLC.cpSTLCa_Defs.
 Require Import ConceptParams.cpSTLC.cpSTLCa_Interpreter.
 
@@ -153,11 +151,6 @@ Theorem ids_are_unique__complete : forall (l : list id),
 Proof.
   apply IdLS.Props.ids_are_unique__complete.
 Qed.
-
-
-
-Section IdSetProofs.
-
 
 (* ----------------------------------------------------------------- *)
 (** **** Types Validity *)
@@ -283,8 +276,6 @@ Proof.
   apply types_valid_b__complete. assumption.
 Qed.
 
-End IdSetProofs.
-
 (* ----------------------------------------------------------------- *)
 (** **** Concept Typing *)
 (* ----------------------------------------------------------------- *)
@@ -295,13 +286,18 @@ End IdSetProofs.
 (** Similarly to IdSets, we need some auxiliary 
   * lemmas to connect AVL maps with lists presenting AST. *)
 
-Module IdMapFacts := FMapFacts.WFacts IdMap.
-Module IdMapProps := FMapFacts.WProperties IdMap.
+(*
+
+*)
+
+Module IdLPMProps := IdLPM.Props.
+Module IdMapFacts := FMapFacts.WFacts IdLPM.IdMap.
+Module IdMapProps := FMapFacts.WProperties IdLPM.IdMap.
 
 Section IdMapProofs.
-
-Import IdMapFacts.
-Import IdMapProps.
+  Import IdLPMProps.
+  Import IdMapFacts.
+  Import IdMapProps.
 
 Lemma split_fst__map_fst : forall {A B : Type} (l : list (prod A B)) 
                                   (xs : list A) (ys : list B),
@@ -322,367 +318,10 @@ Proof.
       apply IHl' with (ys := l0). reflexivity.
 Qed.
 
-Lemma map_from_list_not_in__preserves_mapping : 
-  forall (pnds : list (prod id ty)) (nm : id) (tp : ty)(m : id_map ty),  
-(* JB | cannot figure out how to write [list (id * type)], scoping problems *)
-    IdMap.MapsTo nm tp m ->
-    ~ List.In nm (map fst pnds) ->
-    IdMap.MapsTo nm tp (map_from_list' pnds m).
-Proof.
-  intros pnds. induction pnds as [| pnd pnds' IHpnds'].
-  - (* pnds = nil *)
-    intros nm tp m Hmaps Hnin. simpl. assumption. 
-  - (* pnds = pnd :: pnds' *)
-    intros nm tp m Hmaps Hin.
-    unfold map_from_list' in *. simpl. simpl in IHpnds'.
-    apply IHpnds'.
-    + (* IdMap.MapsTo nm tp (m += pnd) *)    
-      destruct pnd as [x v]. destruct (beq_idP nm x). subst.
-      assert (contra: List.In x (map fst ((x, v) :: pnds'))) 
-        by (simpl; left; reflexivity).
-      apply Hin in contra. contradiction.
-      apply IdMap.add_2. intros H. symmetry in H. apply n in H. 
-      contradiction.
-      assumption.
-    + (* ~ List.In nm (map fst pnds') *)
-      intros H. 
-      assert (contra: List.In nm (map fst (pnd :: pnds')))
-        by (simpl; right; assumption).
-      apply Hin in contra. contradiction.
-Qed.
-
-Lemma map_from_list_add_unique__preserves_mapping : 
-  forall (pnds : list (prod id ty)) (nm : id) (tp : ty) (m : id_map ty),  
-(* JB | cannot figure out how to write [list (id * type)], scoping problems *)
-    ~ List.In nm (map fst pnds) ->
-    IdMap.MapsTo nm tp (map_from_list' ((nm, tp) :: pnds) m).
-Proof. 
-  intros pnds nm tp m. intros Hin.
-  simpl. apply map_from_list_not_in__preserves_mapping.
-  apply IdMap.add_1. reflexivity.
-  assumption.
-Qed.
-
-(*
-IdMap.add_1:
-  forall (elt : Type) (m : IdMap.t elt) (x y : IdMap.key) (e : elt),
-  x = y -> IdMap.MapsTo y e (IdMap.add x e m)
-
-IdMap.find_1:
-  forall (elt : Type) (m : IdMap.t elt) (x : IdMap.key) (e : elt),
-  IdMap.MapsTo x e m -> IdMap.find (elt:=elt) x m = Some e
-*)
-
-Lemma map_from_list__find_cons__true : forall (nm : id) (tp : ty) 
-                                              (nds : list namedecl),
-    let pnds := map namedecl_to_pair nds in
-    ~ List.In nm (List.map fst pnds) ->
-    find_ty nm (map_from_list ((nm, tp) :: pnds)) = Some tp.
-Proof.
-  intros nm tp nds. intros pnds. intros Hin.
-  unfold find_ty, mids_find. 
-  apply IdMap.find_1.
-  apply map_from_list_add_unique__preserves_mapping. auto.
-Qed.
-
-Lemma map_from_list'__eq_maps : 
-  forall (pnds : list (id * ty)%type) (nm : id) (tp : ty) (m m': id_ty_map), 
-    IdMap.Equal m' m ->
-    IdMap.MapsTo nm tp (map_from_list' pnds m)
-    -> 
-    IdMap.MapsTo nm tp (map_from_list' pnds m').
-Proof.
-  intros pnds. induction pnds as [|pnd pnds' IHpnds'].
-  - (* pnds = nil *)
-    intros nm tp m m' Heq Hmaps. 
-    simpl in *. 
-    eapply Equal_mapsto_iff; eauto.
-  - (* pnds = pnd :: pnds' *)
-    intros nm tp m m' Heq Hmaps.
-    destruct pnd as [x v]; simpl in *.
-    eapply IHpnds'.
-    assert (H : IdMap.Equal (mids_add ty x v m') (mids_add ty x v m)).
-    { apply add_m; tauto. }
-    eassumption.
-    assumption.
-Qed.
-
-Lemma permute_add__eq_maps :
-  forall (nm x : id) (tp v : ty) (m : id_ty_map), 
-  x <> nm ->
-  IdMap.Equal (mids_add ty x v (mids_add ty nm tp m))
-              (mids_add ty nm tp (mids_add ty x v m)).
-Proof.
-  intros nm x tp v m Hneq.
-  apply Equal_mapsto_iff.
-  intros k e. split.
-    + intros H1.
-      apply add_mapsto_iff in H1; propositional.
-      subst. apply add_mapsto_iff.
-      right.
-      pose proof (eq_id_dec nm k) as Hid.
-      inversion Hid. subst. simpl in *.
-      assert (contra : k = k) by reflexivity.
-      apply Hneq in contra.
-      contradiction.
-      split; auto.
-      apply add_mapsto_iff.
-      left. split; auto.
-      apply add_mapsto_iff in H1; propositional.
-      subst. apply add_mapsto_iff.
-      left. split; reflexivity.
-      apply add_mapsto_iff.
-      right. split; auto.
-      apply add_mapsto_iff.
-      right. split; auto.
-    + intros H1.
-      apply add_mapsto_iff in H1; propositional.
-      subst. apply add_mapsto_iff.
-      right.
-      pose proof (eq_id_dec x k) as Hid.
-      inversion Hid. subst. simpl in *.
-      assert (contra : k = k) by reflexivity.
-      apply Hneq in contra.
-      contradiction.
-      split; auto.
-      apply add_mapsto_iff.
-      left. split; auto.
-      apply add_mapsto_iff in H1; propositional.
-      subst. apply add_mapsto_iff.
-      left. split; reflexivity.
-      apply add_mapsto_iff.
-      right. split; auto.
-      apply add_mapsto_iff.
-      right. split; auto.
-Qed.
-
-Lemma map_from_list'__ignore_list_add :
-  forall (pnds : list (id * ty)%type) (nm : id) (tp : ty) (m : id_ty_map),  
-  ~ List.In nm (map fst pnds) ->
-  IdMap.MapsTo nm tp (map_from_list' pnds (mids_add ty nm tp m)).
-Proof.
-  intros pnds. induction pnds as [|pnd pnds' IHpnds'].
-  - intros. simpl.
-    apply IdMap.add_1. reflexivity.
-  - intros nm tp m H.
-    destruct pnd as [x v]. simpl. 
-    apply map_from_list'__eq_maps with
-      (m := (mids_add ty nm tp (mids_add ty x v m))).
-    apply permute_add__eq_maps.
-    simpl in H. unfold not. intros contra.
-    eapply or_introl in contra.
-    apply H in contra. contradiction.
-    apply IHpnds'.
-    unfold not in *. intros contra.
-    assert (H1 : List.In nm (map fst ((x, v) :: pnds')))
-      by (simpl; right;  assumption).
-    tauto.
-Qed.
-
-Lemma map_from_list'__ignore_list' :
-  forall (pnds : list (id * ty)%type) (nm : id) (tp : ty) (m : id_ty_map),  
-  ~ List.In nm (map fst pnds) ->
-  IdMap.MapsTo nm tp m ->
-  IdMap.MapsTo nm tp (map_from_list' pnds m).
-Proof.
-  intros pnds. induction pnds as [|pnd pnds' IHpnds'].
-  - intros. simpl. assumption.
-  - intros nm tp m Hin Hmaps.
-    destruct pnd as [x v]. simpl. 
-    apply IHpnds'.
-    simpl in Hin. unfold not in *.
-    intros H.
-    assert (contra : x = nm \/ List.In nm (map fst pnds'))
-      by (right; assumption).
-    tauto.
-    apply add_mapsto_iff.
-    pose proof (eq_id_dec x nm) as Heq. inversion Heq.
-    unfold not in *. simpl in *.
-    assert (contra : x = nm \/ List.In nm (map fst pnds'))
-      by (left; assumption).
-    tauto.
-    right. split; auto.
-Qed.
-
-Lemma map_from_list'__ignore_list :
-  forall (pnds : list (id * ty)%type) (nm : id) (tp : ty) (m : id_ty_map),  
-  ~ List.In nm (map fst pnds) ->
-  IdMap.MapsTo nm tp (map_from_list' pnds m) ->
-  IdMap.MapsTo nm tp m.
-Proof.
-  intros pnds. induction pnds as [|pnd pnds' IHpnds'].
-  - intros. simpl in *. assumption.
-  - intros nm tp m Hin Hmaps.
-    destruct pnd as [x v]. simpl in *. 
-    assert (Hin' : ~ List.In nm (map fst pnds')).
-    { unfold not in *. intros contra.
-      apply Hin. tauto. }  
-    specialize (IHpnds' nm tp (mids_add ty x v m) Hin' Hmaps).
-    apply add_mapsto_iff in IHpnds'.
-    inversion IHpnds'.
-    tauto.
-    tauto.
-Qed.
-
-Lemma map_from_list__any_map : 
-  forall (pnds : list (id * ty)%type) (nm : id) (tp : ty) (m m' : id_ty_map),  
-    List.In nm (map fst pnds) ->
-    (*List.NoDup (map fst pnds)  -> *)
-    IdMap.MapsTo nm tp (map_from_list' pnds m) ->
-    IdMap.MapsTo nm tp (map_from_list' pnds m').
-Proof.
-  intros pnds. induction pnds as [|pnd pnds' IHpnds'].
-  - (* pnds = nil *)
-    intros nm tp m m' Hin (* Hdup *) Hmaps. 
-    simpl in Hin. contradiction.
-  - (* pnds = pnd :: pnds' *)
-    intros nm tp m m' Hin (* Hdup *) Hmaps.
-    simpl. simpl in Hmaps.
-    destruct pnd as [x v].       
-    pose proof (in_dec eq_id_dec nm (map fst pnds')) as Hindec.
-    inversion Hindec as [Hinnm | Hinnm].
-    + eapply IHpnds'.
-      assumption.
-      eassumption.
-    + simpl in Hin. inversion Hin.
-      { subst.
-        pose proof (map_from_list'__ignore_list 
-                      pnds' nm tp (mids_add ty nm v m) Hinnm Hmaps) as Hnm.
-        apply add_mapsto_iff in Hnm; propositional.
-        subst.
-        apply map_from_list'__ignore_list_add.
-        assumption. } 
-      tauto.
-Qed.
-
-Lemma elem_in_map'__elem_in_list' :
-  forall (pnds : list (id * ty)%type) (nm : id) (tp : ty) (m : id_ty_map),
-    IdMap.MapsTo nm tp
-                 (map_from_list' pnds m) ->
-    ~ (IdMap.In nm m) ->
-    List.In nm (map fst pnds).
-Proof.
-  intros pnds. 
-  induction pnds as [| pnd pnds' IHpnds'].
-  - intros. simpl in H. 
-    apply IdMap.find_1 in H.
-    assert (Hfind : IdMap.find (elt:=ty) nm m <> None).
-    equality.    
-    rewrite <- in_find_iff in Hfind.
-    apply H0 in Hfind. contradiction.
-  - intros. destruct pnd as [x v].
-    simpl in *.
-    destruct (beq_idP nm x).
-    + equality.
-    + right.
-      apply IHpnds' with (tp := tp) (m := (mids_add ty x v m)).
-      assumption.
-      unfold "~". intro Hin.
-(*
-add_in_iff:
-  forall (elt : Type) (m : IdMap.t elt) (x y : IdMap.key) (e : elt),
-  IdMap.In (elt:=elt) y (IdMap.add x e m) <-> x = y \/ IdMap.In (elt:=elt) y m
-*)      
-      rewrite add_in_iff in Hin.
-      inversion Hin. equality.
-      apply H0 in H1.
-      assumption.
-Qed.
-
-Lemma elem_in_map'__elem_in_list :
-  forall (pnds : list (id * ty)%type) (nm : id) (tp : ty),
-    IdMap.MapsTo nm tp
-                 (map_from_list' pnds (mids_empty ty)) ->
-    List.In nm (map fst pnds).
-Proof.
-  intros pnds nm tp Hmaps.
-  apply elem_in_map'__elem_in_list' with (tp := tp) (m := (mids_empty ty)).
-  assumption.
-  unfold not. 
-  intros contra. rewrite empty_in_iff in contra.
-  assumption.
-Qed.
-
-Lemma map_from_list'_preserves_eq :
-  forall (pnds : list (id * ty)%type) (m m' : id_ty_map),
-    IdMap.Equal m m' ->
-    IdMap.Equal (map_from_list' pnds m) (map_from_list' pnds m').
-Proof.
-  intros pnds. induction pnds as [|pnd pnds' IHpnds'].
-  - (* pnds = nil *)
-    intros m m' Heq. simpl.
-    assumption.
-  - (* pnds = pnd :: pnds' *)
-    intros m m' Heq. destruct pnd as [x v].
-    simpl.
-    apply IHpnds'.
-    apply F.add_m; tauto.
-Qed.
-
-Lemma map_from_list_cons_cardinal' :
-  forall (pnds : list (id * ty)%type) (nm : id) (tp : ty) (m : id_ty_map),
-    ~ List.In nm (map fst pnds) ->
-    ~ IdMap.In nm m ->
-    IdMap.cardinal (elt:=ty) (map_from_list' ((nm, tp) :: pnds) m)
-    = S (IdMap.cardinal (elt:=ty) (map_from_list' pnds m)).
-Proof.
-  intros pnds. induction pnds as [|pnd pnds' IHpnds'].
-  - (* pnds = nil *)
-    intros nm tp m Hin Hmap. simpl.
-    rewrite <- cardinal_2 with (m' := (mids_add ty nm tp m))
-                              (x := nm) (e := tp).
-    reflexivity.
-    assumption.
-    unfold Add. intros y.
-    reflexivity.
-  - (* pnds = pnd :: pnds' *)
-    intros nm tp m Hin Hmap. destruct pnd as [x v].
-    simpl in *.
-    assert (Heq : IdMap.Equal 
-                    (map_from_list' pnds' (mids_add ty x v (mids_add ty nm tp m)))
-                    (map_from_list' pnds' (mids_add ty nm tp (mids_add ty x v m)))).
-    { apply map_from_list'_preserves_eq.
-      apply permute_add__eq_maps.
-      tauto. }
-    rewrite Heq.
-    apply IHpnds'.
-    tauto. 
-    unfold not. intros contra.
-    rewrite F.add_in_iff in contra.
-    inversion contra; tauto.
-Qed.
-
-Lemma map_from_list_cons_cardinal :
-  forall (pnds : list (id * ty)%type) (nm : id) (tp : ty),
-    ~ List.In nm (map fst pnds) ->
-    IdMap.cardinal (elt:=ty) (map_from_list ((nm, tp) :: pnds))
-    = S (IdMap.cardinal (elt:=ty) (map_from_list pnds)).
-Proof.
-  intros pnds. induction pnds as [|pnd pnds' IHpnds'].
-  - (* pnds = nil *)
-    intros nm tp Hin. 
-    reflexivity.
-  - (* pnds = pnd :: pnds' *)
-    intros nm tp Hin. destruct pnd as [x v].
-    assert (Heq : 
-    IdMap.cardinal (elt:=ty) (map_from_list ((nm, tp) :: (x, v) :: pnds'))
-    = S (IdMap.cardinal (elt:=ty) (map_from_list ((x, v) :: pnds')))).
-    { change (IdMap.cardinal (elt:=ty) 
-                (map_from_list' ((nm, tp) :: (x, v) :: pnds') (mids_empty ty)) 
-              =
-              S (IdMap.cardinal (elt:=ty) (
-                   map_from_list' ((x, v) :: pnds') (mids_empty ty)))).
-      apply map_from_list_cons_cardinal'.
-      assumption.
-      unfold not. intros contra.
-      rewrite F.empty_in_iff in contra. 
-      tauto. }
-    rewrite Heq.
-    unfold map_from_list in *. reflexivity.
-Qed.
+(* ----------------------------------------------------------------- *)
 
 Lemma concept_welldefined_b__cons :
-  forall cst Cnm nd nds,
+  forall (cst : cptcontext) (Cnm : id) (nd : namedecl) (nds : list namedecl),
     concept_welldefined_b cst (cpt_def Cnm (nd :: nds)) = true ->
     concept_welldefined_b cst (cpt_def Cnm nds) = true.
 Proof.
@@ -700,44 +339,8 @@ Proof.
     apply andb_true_iff in H1; propositional.
 Qed.
 
-(* ----------------------------------------------------------------- *)
-
-Lemma in_list__in_map_from_list' :
-  forall (pnds : list (id * ty)%type) (nm : id) (tp : ty) (m : id_ty_map),
-    NoDup (map fst pnds) ->
-    List.In (nm, tp) pnds ->
-    IdMap.MapsTo nm tp (map_from_list' pnds m). 
-Proof.
-  intros pnds. induction pnds as [|pnd pnds' IHpnds'].
-  - (* pnds = nil *)
-    intros nm tp m Hdup Hin. simpl in *.
-    contradiction.
-  - (* pnds = pnd :: pnds' *)
-    intros nm tp m Hdup Hin. destruct pnd as [x v].
-    simpl.
-    inversion Hdup.
-    inversion Hin.
-    inversion H3. subst.
-      apply map_from_list'__ignore_list_add.
-      unfold not. intros contra.
-      tauto.
-    apply IHpnds'; tauto.
-Qed.
-
-Lemma in_list__in_map_from_list :
-  forall (pnds : list (id * ty)%type) (nm : id) (tp : ty),
-    NoDup (map fst pnds) ->
-    List.In (nm, tp) pnds ->
-    IdMap.MapsTo nm tp (map_from_list pnds). 
-Proof.
-  intros.
-  change (IdMap.MapsTo nm tp (map_from_list' pnds (mids_empty ty))).
-  apply in_list__in_map_from_list'; assumption.
-Qed.
-
-
 Lemma concept_welldefined__cons : 
-  forall cst Cnm nd nds,
+  forall (cst : cptcontext) (Cnm : id) (nd : namedecl) (nds : list namedecl),
     concept_welldefined cst (cpt_def Cnm (nd :: nds)) ->
     concept_welldefined cst (cpt_def Cnm nds).
 Proof.
@@ -751,112 +354,89 @@ Proof.
   inversion H1; propositional.
 Qed.
 
-Lemma list_elems_in_map__remove_unused :
-  forall nds f CT CT',
-    Forall
-      (fun nmdecl : namedecl =>
-         match nmdecl with
-         | nm_decl f T => find_ty f CT = Some T
-         end) nds ->
-    ~ In f (map fst (map namedecl_to_pair nds)) ->
-    CT' = IdMap.remove (elt:=ty) f CT ->
-    Forall
-      (fun nmdecl : namedecl =>
-         match nmdecl with
-         | nm_decl f0 T0 => find_ty f0 CT' = Some T0
-         end) nds.
+(* ----------------------------------------------------------------- *)
+
+(** As our IdLPM framework works with list of pairs, and
+    our syntax tree contains [namedecl] instead of pairs,
+    we need a way to convert [namedecl] to pair. *)
+
+Definition namedecl_prop (P : id -> ty -> Prop) :=
+  fun nmdecl : namedecl => 
+    match nmdecl with 
+    | nm_decl f T => P f T 
+    end. 
+Definition namedecl_pair_prop (P : id -> ty -> Prop) :=
+  fun pnd : id * ty => 
+    match pnd with 
+    | (f, T) => P f T 
+    end.
+
+Lemma namedecl_prop__pair : 
+  forall (P : id -> ty -> Prop) (nd : namedecl),
+    namedecl_prop P nd ->
+    namedecl_pair_prop P (namedecl_to_pair nd).
 Proof.
-  intros nds. induction nds as [| nd nds' IHnds' ].
-  - (* nds = nil *)
-    intros f CT CT' Htypes Hin Heq.
-    constructor.
-  - (* nds = nd :: nds' *)
-    intros f CT CT' Htypes Hin Heq.
-    destruct nd as [nm tp]. simpl in *.
-    inversion Htypes; clear Htypes; subst.
-    apply Forall_cons.
-    + pose proof (eq_id_dec nm f).
-      inversion H.
-      { eapply or_introl in H0.
-        eapply Hin in H0. contradiction. }
-      clear H.
-      apply F.find_mapsto_iff.
-      apply F.remove_mapsto_iff.
-      split. equality.
-      apply F.find_mapsto_iff. assumption.
-    + apply IHnds' with (f := f) (CT := CT).
-      assumption.
-      unfold not. intros contra.
-      eapply or_intror in contra.
-      apply Hin in contra. contradiction.
-      reflexivity.
+  intros P nd H. destruct nd as [f T].
+  simpl. assumption.
+Qed.
+Lemma pair_prop__namedecl : 
+  forall (P : id -> ty -> Prop) (nd : namedecl),
+    namedecl_pair_prop P (namedecl_to_pair nd) ->
+    namedecl_prop P nd.
+Proof.
+  intros P nd H. destruct nd as [f T].
+  simpl in *. assumption.
 Qed.
 
-Lemma nd_in_map__nd_in_list :
-  forall nds nm tp CT,
-    Forall
-      (fun nmdecl : namedecl =>
-         match nmdecl with
-         | nm_decl f T => find_ty f CT = Some T
-         end) 
-      nds ->
-    NoDup (map fst (map namedecl_to_pair nds)) ->
-    length nds = IdMap.cardinal (elt:=ty) CT ->
-    IdMap.MapsTo nm tp CT ->
-    List.In (nm_decl nm tp) nds.    
+Lemma forall_namedecl__forall_pair : 
+  forall (P : id -> ty -> Prop) (nds : list namedecl),
+    Forall (namedecl_prop P) nds ->
+    Forall (namedecl_pair_prop P) (map namedecl_to_pair nds).
 Proof.
-  intros nds. induction nds as [| nd nds' IHnds' ].
-  - (* nds = nil *)
-    intros nm tp CT Htypes Hdup Hcard Hmaps. simpl in *.
-    symmetry in Hcard. apply cardinal_Empty in Hcard. 
-    unfold IdMap.Empty in *.
-    unfold IdMap.AvlProofs.Raw.Proofs.Empty in *.
-    apply Hcard in Hmaps; contradiction.
-  - (* nds = nd :: nds' *)
-    intros nm tp CT Htypes Hdup Hcard Hmaps.
-    inversion Htypes; subst; simpl in *. clear Htypes.
-    destruct nd as [f T].
-    simpl in Hdup. inversion Hdup. subst.
-    assert (Hfind := Hmaps).
-    rewrite (F.find_mapsto_iff CT nm tp) in Hfind.
-    unfold find_ty, mids_find in H1.
-    pose proof (eq_id_dec f nm).
-    inversion H; clear H.
-    + subst.
-      rewrite -> H1 in Hfind. inversion Hfind.
-      left; trivial.
-    + right.
-      (* To apply IH, we need smaller map *)
-      remember (IdMap.remove f CT) as CT'.
-      apply IHnds' with (CT := CT').
-      subst CT'.
-      apply list_elems_in_map__remove_unused with (f := f) (CT := CT); trivial.
-      assumption.
-      assert (Hnotin : ~ IdMap.In f CT').
-      { subst. intros contra.
-        apply F.remove_in_iff in contra.
-        inversion contra; tauto. }
-      assert (Hcard' : IdMap.cardinal (elt:=ty) CT 
-                       = S (IdMap.cardinal (elt:=ty) CT')).
-      { apply cardinal_2 with (x := f) (e := T).
-        assumption. unfold Add. subst.
-        intros y. 
-        pose proof (eq_id_dec f y) as Hyf. inversion Hyf.
-        subst.
-        rewrite H1. 
-        rewrite (F.add_eq_o _ _ (eq_refl y)). reflexivity.
-        rewrite (F.add_neq_o _ _ H).
-        symmetry. apply F.remove_neq_o. assumption. }
-      rewrite <- Hcard in Hcard'.
-      inversion Hcard'. reflexivity.
-      subst. apply F.remove_neq_mapsto_iff. assumption. assumption.
-Qed.      
+  intros P nds. induction nds as [| nd nds' IHnds'].
+  - intros _. simpl. constructor.
+  - intros H. inversion H; subst. 
+    simpl. constructor.
+    apply namedecl_prop__pair; assumption.
+    apply IHnds'; assumption.
+Qed.
+Lemma forall_pair__forall_namedecl : 
+  forall (P : id -> ty -> Prop) (nds : list namedecl),
+    Forall (namedecl_pair_prop P) (map namedecl_to_pair nds) ->
+    Forall (namedecl_prop P) nds.
+Proof.
+  intros P nds. induction nds as [| nd nds' IHnds'].
+  - intros _. simpl. constructor.
+  - intros H. inversion H; subst. 
+    simpl. constructor.
+    apply pair_prop__namedecl; assumption.
+    apply IHnds'; assumption.
+Qed.
+
+Lemma in_pair__in_namedecl : 
+  forall (nds : list namedecl) (nd : namedecl),
+    In (namedecl_to_pair nd) (map namedecl_to_pair nds) ->
+    In nd nds.
+Proof.
+  intros nds. induction nds as [| nd' nds' IHnds'].
+  - intros nd H. inversion H. 
+  - intros nd H. 
+    simpl. simpl in H. 
+    inversion H as [H' | H'].
+    + left. unfold namedecl_to_pair in H'. 
+      cases nd'. cases nd. subst. 
+      inversion H'. subst. reflexivity.
+    + right.    
+      auto.
+Qed.
+
+(* ----------------------------------------------------------------- *)
 
 Lemma concept_has_type_iso : 
   forall (cst : cptcontext) (C : conceptdef) (CT CT' : id_ty_map),  
     concept_has_type cst C (CTdef CT) ->
     concept_has_type cst C (CTdef CT') ->
-    IdMap.Equal CT CT'.
+    IdLPM.IdMap.Equal CT CT'.
 Proof.
   intros cst C. 
   destruct C as [Cnm nmtps].
@@ -866,37 +446,46 @@ Proof.
   - (* nil *)
     simpl in *. symmetry in H4, H5.
     apply cardinal_Empty in H4. apply cardinal_Empty in H5.
-    unfold IdMap.Empty in *.
-    unfold IdMap.AvlProofs.Raw.Proofs.Empty in H4, H5.
+    unfold IdLPM.IdMap.Empty in *.
+    unfold IdLPM.IdMap.Raw.Proofs.Empty in H4, H5.
     apply F.Equal_mapsto_iff.
     intros k e. split; intros contra.
-    + unfold IdMap.MapsTo in contra. apply H4 in contra. contradiction.
-    + unfold IdMap.MapsTo in contra. apply H5 in contra. contradiction.
+    + unfold IdLPM.IdMap.MapsTo in contra. apply H4 in contra. contradiction.
+    + unfold IdLPM.IdMap.MapsTo in contra. apply H5 in contra. contradiction.
   - (* nmtps = nmtp :: nmtps' *)
-
     unfold concept_welldefined in H.
     destruct (split (map namedecl_to_pair (nmtp :: nmtps'))) 
       as [fnames ftypes] eqn:Heq.
     propositional.
     apply split_fst__map_fst in Heq. subst.
-
+    remember (map namedecl_to_pair (nmtp :: nmtps')) as pnds.
     apply F.Equal_mapsto_iff.
-    intros k e. split; intros Hmaps.
-    
-    assert (Hin : List.In (nm_decl k e) (nmtp :: nmtps')).
-    apply nd_in_map__nd_in_list with (CT := CT).
-    assumption. assumption. assumption. assumption.
+    (* IdLPM.IdMap.MapsTo k e CT <-> IdLPM.IdMap.MapsTo k e CT' *)
+    intros k e. split; intros Hmaps;
+                  assert (Hin : List.In (k, e) pnds).
+    (* CT -> CT' *)
+    apply elem_in_map_eq_length__elem_in_list with (CT := CT).
+    subst pnds.
+    apply forall_namedecl__forall_pair. apply H3. assumption. 
+    subst. rewrite map_length. assumption.
+    assumption.
     rewrite Forall_forall in H0.
+    subst. 
+    change (In (namedecl_to_pair (nm_decl k e)) (map namedecl_to_pair (nmtp :: nmtps'))) in Hin.
+    apply in_pair__in_namedecl in Hin.
     specialize (H0 (nm_decl k e) Hin).
-    inversion H0.
     apply F.find_mapsto_iff. assumption.
-
-    assert (Hin : List.In (nm_decl k e) (nmtp :: nmtps')).
-    apply nd_in_map__nd_in_list with (CT := CT').
-    assumption. assumption. assumption. assumption.
+    (* CT' -> CT *)
+    apply elem_in_map_eq_length__elem_in_list with (CT := CT').
+    subst pnds.
+    apply forall_namedecl__forall_pair. apply H0. assumption. 
+    subst. rewrite map_length. assumption.
+    assumption.
     rewrite Forall_forall in H3.
+    subst. 
+    change (In (namedecl_to_pair (nm_decl k e)) (map namedecl_to_pair (nmtp :: nmtps'))) in Hin.
+    apply in_pair__in_namedecl in Hin.
     specialize (H3 (nm_decl k e) Hin).
-    inversion H3.
     apply F.find_mapsto_iff. assumption.
 Qed.    
 
@@ -938,10 +527,10 @@ Proof.
     apply ids_are_unique__sound in Huniq. 
     apply Forall_cons(*; destruct d; simpl in HCdef*).
     + (* head *)
-      simpl. apply map_from_list__find_cons__true.
+      simpl. apply map_from_list__find_cons___true.
       (* ~ List.In i (map fst (map namedecl_to_pair nds')) *)
       inversion Huniq; subst.
-      replace (map fst (map namedecl_to_pair nds')) with nms.
+      replace (IdLPM.get_ids (map namedecl_to_pair nds')) with nms.
       assumption. 
       apply split_fst__map_fst in eqpnds'. auto.
 (*
@@ -954,22 +543,13 @@ Forall_impl:
       apply Forall_impl with (P := fun nmdecl : namedecl =>
               match nmdecl with
               | nm_decl f T =>
-                  find_ty f (map_from_list (map namedecl_to_pair nds')) = Some T
+                  find_ty f (IdLPM.map_from_list (map namedecl_to_pair nds')) = Some T
               end).
       intros [f T] H.
       simpl.
-      apply IdMap.find_2 in H.
-      apply IdMap.find_1.
-      change (IdMap.MapsTo f T 
-             (map_from_list' ((i, t) :: map namedecl_to_pair nds') 
-                             (mids_empty ty))).
-      change (IdMap.MapsTo f T 
-             (map_from_list' (map namedecl_to_pair nds') 
-                             (mids_empty ty))) in H.
-      simpl.
-      apply map_from_list__any_map with (m := (mids_empty ty)).     
-      apply elem_in_map'__elem_in_list with (tp := T).
-      assumption. assumption.
+      apply IdLPM.IdMap.find_2 in H.
+      apply IdLPM.IdMap.find_1. 
+      apply map_from_list_cons__preserves_mapping. assumption.
       (* forall implication *)
       inversion Huniq; subst; simpl in *.
       apply IHnds'.
@@ -985,25 +565,14 @@ Forall_impl:
       inversion H0. inversion eqpnds'. subst.
       assumption.
   - (* length *)
-    induction nds as [| d nds' IHnds']. 
-    reflexivity.
-    destruct d as [nm tp].
-    simpl.
-    rewrite map_from_list_cons_cardinal.
-    apply f_equal.
-    apply IHnds'.
-    apply concept_welldefined_b__cons with (nd := nm_decl nm tp); assumption.
-    simpl in Hsound.
-    destruct (split (map namedecl_to_pair nds')) as [fnames ftypes].
-    propositional.
-    inversion H; tauto.
-    inversion H0; tauto.
-    (* ~ List.In *)
-    simpl in Hsound.
-    destruct (split (map namedecl_to_pair nds')) as [fnames ftypes] eqn:Heq.
-    propositional.
-    inversion H0. apply split_fst__map_fst in Heq. subst.
-    tauto.
+    remember (map namedecl_to_pair nds) as pnds.
+    assert (Hlen : length pnds = length nds).
+    { subst pnds. rewrite map_length. reflexivity. }
+    rewrite <- Hlen.
+    apply map_from_list__length_cardinal_eq.
+    destruct (split pnds) as [fnames ftypes] eqn:Hpnds; propositional.
+    apply split_fst__map_fst in Hpnds.
+    unfold IdLPM.get_ids. subst fnames. assumption.
 Qed.
 
 (** Here is the main [concept_type_check] completeness theorem. *)
@@ -1012,41 +581,12 @@ Theorem concept_type_check__complete :
   forall (cst : cptcontext) (C : conceptdef) (CT CT' : id_ty_map),  
     concept_has_type cst C (CTdef CT) ->
     concept_type_check cst C = Some (CTdef CT') ->
-    IdMap.Equal CT CT'.
+    IdLPM.IdMap.Equal CT CT'.
 Proof.
   intros cst C CT CT' Hhas Hcheck.
   apply concept_type_check__sound in Hcheck.
   apply concept_has_type_iso with (cst := cst) (C := C);
     assumption.
-(*
-  (* simplify [has] hypothesis *)
-  destruct C as [Cnm nds].
-  unfold concept_has_type in Hhas.
-  inversion Hhas as [Hwell Hbody]. clear Hhas.
-  inversion Hbody as [Htys Hlen]. clear Hbody.
-  (* simplify [check] hypothesis *)
-  unfold concept_type_check in Hcheck.
-  pose proof (concept_well_defined_b__complete _ _ Hwell) as Hwell'.
-  rewrite Hwell' in Hcheck.
-  inversion Hcheck as [Hcheck']. clear Hcheck. 
-  (* Main goal: map_from_list (map namedecl_to_pair nds) = nmtps *)
-
-  unfold concept_welldefined in Hwell.
-  destruct (split (map namedecl_to_pair nds)) as [fnames ftypes] eqn:Hnds.
-  assert (Hnds' := Hnds).
-  apply split_fst__map_fst in Hnds. subst.
-  inversion Hwell as [Hdup Htys'].
-
-  apply F.Equal_mapsto_iff.
-  intros k e.
-  repeat rewrite -> F.find_mapsto_iff.
-  split.
-  + intros H.
-    unfold concept_welldefined_b in Hwell'.
-    rewrite <- F.find_mapsto_iff.
-    apply in_list__in_map_from_list.
-    assumption.
- *)   
 Qed.
 
 End IdMapProofs.
