Makefile
@@ -102,8 +102,8 @@ VFILES:=BasicPLDefs/Identifier.v\
   BasicPLDefs/Utils.v\
   AuxTactics/LibTactics.v\
   AuxTactics/BasicTactics.v\
-  ListAsAVL/ListAsSet.v\
-  ListAsAVL/ListPairAsMap.v\
+  List2AVL/List2Set.v\
+  List2AVL/ListPair2Map.v\
   cpSTLC/cpSTLCa_Defs.v\
   cpSTLC/cpSTLCa_Interpreter.v\
   cpSTLC/cpSTLCa_Examples.v\
